Fix a number of extraction issues
Need to avoid using module aliases since they generate new copies of
inductives; possibly related to https://github.com/coq/coq/issues/8152.

logging-client/fiximports.py
@@ -11,31 +11,6 @@ import_modules = {
     [
         "Disk",
     ],
-
-    "import qualified Replication.TwoDiskOps":
-    [
-        "TwoDiskBaseImpl",
-    ],
-
-    "import Replication.TwoDiskEnvironment":
-    [
-        "ReplicatedDiskImpl",
-        "NbdImpl",
-        "NbdServer",
-        "ReplicatedServer",
-        "TwoDiskBaseImpl",
-        "Abstraction",
-    ],
-
-    "import qualified Data.Word":
-    [
-        "NbdAPI",
-    ],
-
-    "import qualified Network.ServerOps":
-    [
-        "NbdImpl",
-    ],
 }
 
 module_imports = {}
