logging-client/src/Main.hs
@@ -12,22 +12,13 @@ data InitOptions = InitOptions
   { defaultSizeKB :: Int
   , initDiskPaths :: (FilePath, FilePath) }
 
-data Options = Start ServerOptions
-             | Init InitOptions
+data Options = Init InitOptions
 
 parseDiskPaths :: Parser (FilePath, FilePath)
 parseDiskPaths = ((,)
                 <$> argument str (metavar "FILE0")
                 <*> argument str (metavar "FILE1"))
                <|> pure ("disk0.img", "disk1.img")
-
-serverOptions :: Parser ServerOptions
-serverOptions = do
-  diskPaths <- parseDiskPaths
-  logCommands <- switch (long "debug"
-                        <> short 'd'
-                        <> help "log each operation received")
-  pure ServerOptions {..}
 
 initOptions :: Parser InitOptions
 initOptions = do
@@ -45,10 +36,7 @@ diskDefaultMessage = "disks default to disk0.img and disk1.img if not provided"
 
 options :: Parser Options
 options = hsubparser
-          ( command "start" (info (Start <$> serverOptions)
-                             (progDesc "start server"
-                             <> footer diskDefaultMessage))
-            <> command "init" (info (Init <$> initOptions)
+          ( command "init" (info (Init <$> initOptions)
                                (progDesc "initialize replicated disks"
                                <> footer diskDefaultMessage))
           )
@@ -58,22 +46,20 @@ main = execParser opts >>= run
   where
     opts = info (options <**> helper)
       (fullDesc
-       <> progDesc "an nbd server that replicates over two disks; COMMAND is either init or start"
-       <> header "replicate-nbd - replicating network block device"
+       <> progDesc "logging over replicated disks"
+       <> header "logging-client: example of using logging over replication"
        )
 
 run :: Options -> IO ()
-run (Start opts) = runServer opts
 run (Init opts) = runInit opts
 
 runInit :: InitOptions -> IO ()
 runInit InitOptions
   { defaultSizeKB=size,
-    initDiskPaths=diskPaths@(fn0, fn1) } = do
+    initDiskPaths=(fn0, fn1) } = do
   exists0 <- doesFileExist fn0
   exists1 <- doesFileExist fn1
   when (not exists0 && not exists1) $
     forM_ [fn0, fn1] $ \p ->
       withFile p WriteMode $ \h ->
         hSetFileSize h (fromIntegral $ size * 1024)
-  initServer diskPaths
